specs/Spec.Kraft.fsti
@@ -1,0 +1,14 @@
+module Spec.Kraft
+
+open FStar.Seq
+open Lib.Rational
+open Lib.Seq
+
+let rec kraft_sum (l: seq nat): Tot rat (decreases length l) =
+  match length l with
+  | 0 -> zero
+  | _ -> qpow2 (-l.[0]) +$ kraft_sum (tail l)
+
+type kraft_series (max_len: pos) = l: seq nat{
+  kraft_sum l =$ one /\ (forall i. l.[i] <= max_len)
+}
